finish the correctness part of the proof for copy_insert.
Do this by changing the correctness condition for copy_insert
to be in terms of SequenceR instead of IndexR.

It would be good to prove the two conditions are the same at some
point but it is too annoying to do now

logical/sequence.v
@@ -100,3 +100,22 @@ Proof.
   apply IH in IN; destruct IN as [i IR]; eauto.
 Qed.
 Hint Resolve SequenceR_In.
+
+Fixpoint mk_list {A:Set} (x:A) (n:nat) :=
+  match n with
+    | 0 => nil
+    | S n' => cons x (mk_list x n')
+  end.
+
+Lemma interleave_mk_list_same_size : 
+  forall (A:Set) (x:A) n,
+    interleave (mk_list x n) (mk_list x n) = mk_list x (n+n).
+  induction n; auto.
+  simpl.
+  rewrite <- interleave_case2.
+  rewrite <- interleave_case2.
+  rewrite IHn.
+  replace (n + S n) with (S (n + n)); try omega.
+  auto.
+Qed.
+
