tmonad/copy_insert.v
@@ -1,5 +1,6 @@
 Require Import Braun.tmonad.monad Braun.logical.index Braun.tmonad.insert.
 Require Import Braun.common.braun Braun.common.util Braun.common.big_oh.
+Require Import Braun.logical.list_util.
 Require Import Braun.logical.sequence.
 Require Import Arith Arith.Even Arith.Div2 Omega.
 Require Import Program.Wf.
@@ -8,7 +9,7 @@ Definition copy_insert_time (n:nat) := 3.
 
 Definition copy_insert_result (A:Set) (x:A) (n:nat) (b:@bin_tree A) (c:nat):=
   Braun b n /\ 
-  (forall i y, IndexR b i y -> y = x) /\
+  SequenceR b (mk_list x n) /\
   c = copy_insert_time (n).
 
 Load "copy_insert_gen.v".
@@ -16,17 +17,16 @@ Load "copy_insert_gen.v".
 Next Obligation.
   unfold copy_insert_result.
   repeat constructor; auto.
-  
-  intros i y IR.
-  inversion IR.
 Qed.
 
 Next Obligation.
+  clear copy_insert.
   clear am H2.
   rename H1 into CIR.
   rename H into EVENNPRIME.
 
   inversion CIR as [BRAUNT [HIR TIME]].
+  clear CIR.
 
   unfold copy_insert_result.
   repeat split.
@@ -39,13 +39,12 @@ Next Obligation.
   constructor; auto; try omega.
 
   (* correct *)
-  intros i y IR.
-  invclr IR; auto.
-  remember (HIR i0 y H4).
-  auto.
-
-  remember (HIR i0 y H4).
-  auto.
+  simpl.
+  replace (mk_list x n') with (interleave (mk_list x (div2 n')) (mk_list x (div2 n'))).
+  apply SR_node; auto.
+  replace (mk_list x n') with (mk_list x (div2 n'+div2 n')).
+  apply interleave_mk_list_same_size.
+  rewrite -> (even_double n') at 3; auto.
 
   (* running time *)
   admit.
@@ -75,10 +74,23 @@ Next Obligation.
   rewrite <- (odd_double n'); auto; try omega.
 
   (* correctness *)
-  intros i y IR.
-  invclr IR; auto.
-  admit. (* the case when we called insert *)
-  remember (INDEX i0 y H5); auto.
+  remember INDEX as INDEXS. clear HeqINDEXS.
+  apply SEQ in INDEXS.
+  clear SEQ.
+  simpl.
+  replace (mk_list x n') with (interleave (x :: mk_list x (div2 n'))
+                                          (mk_list x (div2 n'))).
+  constructor; auto.
+  replace (mk_list x n') with (mk_list x (div2 n' + div2 n' + 1)).
+  rewrite <- interleave_case2.
+  replace (div2 n'+div2 n'+1) with (S (div2 n'+div2 n')); try omega.
+  simpl.
+  rewrite interleave_mk_list_same_size.
+  reflexivity.
+  rewrite (odd_double n') at 3;auto.
+  unfold double.
+  replace  (div2 n' + div2 n' + 1) with (S (div2 n' + div2 n')); try omega.
+  reflexivity.
 
   (* running time *)
   admit.
